aneris/aneris_lang/state_interp/state_interp_free_ports_coh.v
@@ -18,10 +18,10 @@ Section state_interpretation.
   Context `{!anerisG Mdl Σ}.
 
   Lemma free_ports_coh_init free_ports σ :
-    (map_Forall (λ ip ports,
-                     (∀ Sn, (state_sockets σ) !! ip = Some Sn →
-                            set_Forall (λ p, port_not_in_use p Sn) ports))
-                free_ports) →
+    set_Forall
+      (λ p,
+         (∀ Sn, (state_sockets σ) !! (ip_of_address p) = Some Sn →
+                port_not_in_use (port_of_address p) Sn)) free_ports →
     free_ports_auth free_ports -∗
     free_ports_coh σ.
   Proof. iIntros (?) "?". by iExists _; iFrame. Qed.
@@ -29,13 +29,12 @@ Section state_interpretation.
   Lemma free_ports_coh_free_ports_valid σ a Sn :
     state_sockets σ !! ip_of_address a = Some Sn →
     free_ports_coh σ -∗
-    free_ports (ip_of_address a) {[port_of_address a]} -∗
+    free_ports {[a]} -∗
     ⌜port_not_in_use (port_of_address a) Sn⌝.
   Proof.
     iIntros (Hskts). iDestruct 1 as (ports Hports) "HpCtx". iIntros "Hp".
-    iDestruct (free_ports_included with "HpCtx Hp") as (?) "[%Hlookup %]".
-    iPureIntro.
-    eapply Hports; [done|done|set_solver].
+    iDestruct (free_ports_included with "HpCtx Hp") as "%".
+    iPureIntro. eapply Hports; [set_solver|done].
   Qed.
 
   Lemma free_ports_coh_alloc_node ip σ :
@@ -46,8 +45,8 @@ Section state_interpretation.
     intros Hip.
     iDestruct 1 as (ps Hps) "HpsCtx".
     iExists _. iFrame. iPureIntro.
-    intros ip' ps' HSome' Sn' HPs'.
-    destruct (decide (ip = ip')); simplify_map_eq.
+    intros sa Hin Sn' HPs'.
+    destruct (decide (ip = ip_of_address sa)); simplify_map_eq.
     - intros ???????. set_solver.
     - by eapply Hps.
   Qed.
@@ -65,9 +64,9 @@ Section state_interpretation.
     intros Hip.
     iDestruct 1 as (ps Hps) "HpsCtx".
     iExists _. iFrame. iPureIntro.
-    intros ip' ps' HSome' Sn' HPs'.
-    destruct (decide (ip = ip')); simplify_map_eq.
-    - intros p Hin sh' skt' a' r' Hsh' Haddr.
+    intros sa Hin Sn' HSn'.
+    destruct (decide (ip = ip_of_address sa)); simplify_map_eq.
+    - intros sh' skt' a' r' Hsh' Haddr.
       destruct (decide (sh = sh')) as [->|Hneq].
       + rewrite lookup_insert in Hsh'. simplify_eq.
       + rewrite lookup_insert_ne in Hsh'; [|done]. by eapply Hps.
@@ -88,13 +87,11 @@ Section state_interpretation.
     intros Hskt HSn Hsh.
     iDestruct 1 as (ps Hps) "HpsCtx".
     iExists _. iFrame. iPureIntro.
-    intros ip' ps' HSome' Sn' HPs'.
-    destruct (decide (ip = ip')); simplify_map_eq.
-    - intros p Hin.
-      intros sh' skt' a' r' Hsh' Haddr.
+    intros sa Hin Sn' HSn'.
+    destruct (decide (ip = ip_of_address sa)); simplify_map_eq.
+    - intros sh' skt' a' r' Hsh' Haddr.
       destruct (decide (sh = sh')) as [->|Hneq].
-      + rewrite lookup_insert in Hsh'. simplify_eq. simpl in Haddr.
-        simplify_eq. by eapply Hps.
+      + rewrite lookup_insert in Hsh'. simplify_eq. by eapply Hps.
       + rewrite lookup_insert_ne in Hsh'; [|done]. by eapply Hps.
     - by eapply Hps.
   Qed.
@@ -111,31 +108,31 @@ Section state_interpretation.
                      (state_sockets σ1) |>).
   Proof. iIntros (??) "?". by iApply free_ports_coh_update_socket. Qed.
 
-  Lemma free_ports_coh_bind_socket σ1 a r sh skt Sn :
-    state_sockets σ1 !! ip_of_address a = Some Sn →
+  Lemma free_ports_coh_bind_socket σ1 sa r sh skt Sn :
+    state_sockets σ1 !! ip_of_address sa = Some Sn →
     free_ports_coh σ1 -∗
-    free_ports (ip_of_address a) {[port_of_address a]} ==∗
+    free_ports {[sa]} ==∗
     free_ports_coh
       (σ1 <| state_sockets :=
-         <[ip_of_address a :=
-             <[sh:=(skt<| saddress := Some a |>, r)]> Sn]>
+         <[ip_of_address sa :=
+             <[sh:=(skt<| saddress := Some sa |>, r)]> Sn]>
                  (state_sockets σ1) |>).
   Proof.
     intros HSome.
     iDestruct 1 as (Ps HPs) "HpCtx".
     iIntros "Hp".
-    iMod (free_ports_dealloc with "HpCtx Hp")
-      as (ps [Hps' Hin%elem_of_subseteq_singleton]) "HpCtx".
+    iMod (free_ports_dealloc with "HpCtx Hp") as "HpCtx".
     iModIntro. iExists _; iFrame. iPureIntro.
-    intros ip' ps' HSome' Sn' HPs'.
-    destruct (decide (ip_of_address a = ip')); simplify_map_eq.
-    - intros p [Hin' Hnin%not_elem_of_singleton]%elem_of_difference.
-      intros sh' skt' a' r' Hsh' Haddr. simplify_eq.
+    destruct sa as [ip p].
+    intros [ip' p'] Hin Sn' HSn'.
+    destruct (decide (ip = ip')); simplify_map_eq.
+    - intros sh' skt' a' r' Hsh' Haddr.
       destruct (decide (sh = sh')) as [->|Hneq].
       + rewrite lookup_insert in Hsh'. simplify_eq. simpl in Haddr.
-        by simplify_eq.
-      + rewrite lookup_insert_ne in Hsh'; [|done]. by eapply HPs.
-    - by eapply HPs.
+        simplify_eq. by set_solver.
+      + rewrite lookup_insert_ne in Hsh'; [|done].
+        eapply (HPs (SocketAddressInet ip' p')); try done. set_solver.
+    - eapply (HPs (SocketAddressInet ip' p')); try done. set_solver.
   Qed.
 
   Lemma free_ports_coh_update hps1 hps2 skts ms1 ms2 :
