aneris/examples/minimal_example/minimal_example_proof.v
@@ -239,7 +239,7 @@ Lemma gcounter_adequacy ip :
     {tr[ ([mkExpr ip incr_example], init_state ip) ]}
     {tr[ 0%nat ]}.
 Proof.
-  eapply (simulation_adequacy #[anerisΣ incr_exampleM; GFunctor incr_res] incr_exampleM NotStuck ∅ {["s"]} ∅ ∅ ∅ ∅ (λ _, True) _ ip).
+  eapply (simulation_adequacy #[anerisΣ incr_exampleM; GFunctor incr_res] incr_exampleM NotStuck ∅ {["s"]} ∅ ∅ ∅ (λ _, True) _ ip).
   { set_solver. }
   { set_solver. }
   { apply aneris_sim_rel_finitary, incr_exampleM_finitary. }
